Wrap primitives proto as hoare triples
TODO: use them to prove swap_pair; this requires fixing the way
prog_environs are handled and the various combinators on them

theories/c_interop/rules.v
@@ -1,7 +1,8 @@
 From iris.proofmode Require Import proofmode.
-From melocoton.interop Require Import basics basics_resources gctoken update_laws.
-From melocoton.ml_lang Require Import primitive_laws.
-From melocoton.c_interface Require Export resources.
+From melocoton Require Import named_props.
+From melocoton.interop Require Import basics basics_resources gctoken update_laws prims prims_proto.
+From melocoton.ml_lang Require Import lang_instantiation primitive_laws.
+From melocoton.c_interface Require Export defs resources.
 From melocoton.c_lang Require Import primitive_laws tactics notation proofmode.
 From iris.prelude Require Import options.
 
@@ -18,10 +19,12 @@ Context {Σ : gFunctors}.
 Context `{!heapGS_ML Σ, !heapGS_C Σ, !invGS_gen hlc Σ}.
 Context `{!wrapperGCtokGS Σ}.
 
+(* Reading and writing roots using plain C reads and writes *)
+
 Lemma store_to_root E pe (l:loc) (v v' : lval) w θ :
   repr_lval θ v w →
   {{{ GC θ ∗ l ↦roots v' }}}
-     (#l <- w)%E @ pe; E
+     (#l <- w)%CE @ pe; E
   {{{ RET LitV LitUnit; GC θ ∗ l ↦roots v }}}%CE.
 Proof.
   iIntros (Hrepr Φ) "(HGC&Hroot) HΦ".
@@ -34,13 +37,236 @@ Qed.
 
 Lemma load_from_root E pe (l:loc) (v : lval) dq θ :
   {{{ GC θ ∗ l ↦roots{dq} v }}}
-     ( * #l)%E @ pe; E
+     ( * #l)%CE @ pe; E
   {{{ w, RET w; l ↦roots{dq} v ∗ GC θ ∗ ⌜repr_lval θ v w⌝ }}}%CE.
 Proof.
   iIntros (Φ) "(HGC&Hroot) HΦ".
   iDestruct (access_root with "[$HGC $Hroot]") as (w') "(Hpto & %Hrepr & Hupd)".
   iApply (wp_load with "Hpto"). iIntros "!> Hpto".
   iDestruct ("Hupd" with "Hpto") as "(?&?)". iApply "HΦ". by iFrame.
+Qed.
+
+(* Calling to runtime primitives *)
+
+(* TODO: move / refactor / merge with the other penv combinators *)
+Definition penv_with_prims E (pe : language.weakestpre.prog_environ C_lang Σ) (T : ML_proto Σ) :
+  language.weakestpre.prog_environ C_lang Σ
+  :=
+  {| penv_prog := filter (λ '(s, _), ¬ is_prim_name s) (penv_prog pe);
+     penv_proto := (λ f vs Φ, proto_prims_in_C E T f vs Φ ∨ penv_proto pe f vs Φ)%I; |}.
+
+
+Lemma int2val_spec E pe (T : ML_proto Σ) θ (x : Z) :
+  {{{ GC θ }}}
+    (call: &"int2val" with (Val #x))%CE @ (penv_with_prims E pe T); E
+  {{{ w, RET w; GC θ ∗ ⌜repr_lval θ (Lint x) w⌝ }}}.
+Proof.
+  iIntros (Φ) "HGC Cont".
+  wp_pures. wp_extern.
+  { cbn. apply map_filter_lookup_None_2. right.
+    intros _ _. intros H; apply H. eexists; constructor. }
+  iModIntro. cbn. iLeft. iExists _. iSplit; first by eauto.
+  iLeft. iLeft. rewrite /proto_int2val /named. iExists _, _. iFrame.
+  do 2 (iSplit; first by eauto). iIntros "!>" (?) "HGC %".
+  iApply wp_value; eauto. iApply "Cont"; eauto.
+Qed.
+
+Lemma val2int_spec E pe (T : ML_proto Σ) θ (w:word) (x:Z) :
+  repr_lval θ (Lint x) w →
+  {{{ GC θ }}}
+    (call: &"val2int" with (Val w))%CE @ (penv_with_prims E pe T); E
+  {{{ RET (#x); GC θ }}}.
+Proof.
+  iIntros (Hrepr Φ) "HGC Cont".
+  wp_pures. wp_extern.
+  { cbn. apply map_filter_lookup_None_2. right.
+    intros _ _. intros H; apply H. eexists; constructor. }
+  iModIntro. cbn. iLeft. iExists _. iSplit; first by eauto.
+  iLeft. iRight; iLeft. rewrite /proto_val2int /named. iExists _, _, _. iFrame.
+  do 3 (iSplit; first by eauto). iIntros "!> HGC".
+  iApply wp_value; eauto. iApply "Cont"; eauto.
+Qed.
+
+Lemma registerroot_spec E pe (T : ML_proto Σ) θ v w a :
+  repr_lval θ v w →
+  {{{ GC θ ∗ a ↦C w }}}
+    (call: &"registerroot" with (Val (# a)))%CE
+      @ (penv_with_prims E pe T); E
+  {{{ RET (# 0); GC θ ∗ a ↦roots v }}}.
+Proof.
+  iIntros (Hrepr Φ) "(HGC & Hpto) Cont".
+  wp_pures. wp_extern.
+  { cbn. apply map_filter_lookup_None_2. right.
+    intros _ _. intros H; apply H. eexists; constructor. }
+  iModIntro. cbn. iLeft. iExists _. iSplit; first by eauto.
+  iLeft. do 2 iRight; iLeft. rewrite /proto_registerroot /named.
+  iExists _, _, _, _. iFrame.
+  do 3 (iSplit; first by eauto). iIntros "!> ? ?".
+  iApply wp_value; eauto. iApply "Cont"; eauto. iFrame.
+Qed.
+
+Lemma unregisterroot_spec E pe (T : ML_proto Σ) θ v a :
+  {{{ GC θ ∗ a ↦roots v }}}
+    (call: &"unregisterroot" with (Val (# a)))%CE
+      @ (penv_with_prims E pe T); E
+  {{{ w, RET (# 0); GC θ ∗ a ↦C w ∗ ⌜repr_lval θ v w⌝ }}}.
+Proof.
+  iIntros (Φ) "(HGC & Hpto) Cont".
+  wp_pures. wp_extern.
+  { cbn. apply map_filter_lookup_None_2. right.
+    intros _ _. intros H; apply H. eexists; constructor. }
+  iModIntro. cbn. iLeft. iExists _. iSplit; first by eauto.
+  iLeft. do 3 iRight; iLeft. rewrite /proto_unregisterroot /named.
+  iExists _, _, _. iFrame.
+  do 2 (iSplit; first by eauto). iIntros "!>" (?) "? ? %".
+  iApply wp_value; eauto. iApply "Cont"; eauto. by iFrame.
+Qed.
+
+Lemma modify_spec E pe (T : ML_proto Σ) θ γ w mut tg vs v' w' i :
+  repr_lval θ (Lloc γ) w →
+  vblock_access_le M mut →
+  repr_lval θ v' w' →
+  (0 ≤ i < length vs)%Z →
+  {{{ GC θ ∗ γ ↦vblk[mut] (tg, vs) }}}
+    (call: &"modify" with (Val w, Val (# i), Val w'))%CE
+      @ (penv_with_prims E pe T); E
+  {{{ RET (# 0); GC θ ∗ γ ↦vblk[mut] (tg, <[Z.to_nat i:=v']> vs) }}}.
+Proof.
+  intros. iIntros "(HGC & Hpto) Cont".
+  wp_pures. wp_extern.
+  { cbn. apply map_filter_lookup_None_2. right.
+    intros _ _. intros HH; apply HH. eexists; constructor. }
+  iModIntro. cbn. iLeft. iExists _. iSplit; first by eauto.
+  iLeft. do 4 iRight; iLeft. rewrite /proto_modify /named.
+  do 9 iExists _. iFrame.
+  do 7 (iSplit; first by eauto with lia). iIntros "!> ? ?".
+  iApply wp_value; eauto. iApply "Cont"; eauto. by iFrame.
+Qed.
+
+Lemma readfield_spec E pe (T : ML_proto Σ) θ γ w m dq tg vs i :
+  repr_lval θ (Lloc γ) w →
+  (0 ≤ i < length vs)%Z →
+  {{{ GC θ ∗ γ ↦vblk[m]{dq} (tg, vs) }}}
+    (call: &"readfield" with (Val w, Val (# i)))%CE
+      @ (penv_with_prims E pe T); E
+  {{{ v' w', RET w';
+        GC θ ∗ γ ↦vblk[m]{dq} (tg, vs) ∗
+        ⌜vs !! (Z.to_nat i) = Some v'⌝ ∗
+        ⌜repr_lval θ v' w'⌝ }}}.
+Proof.
+  intros. iIntros "(HGC & Hpto) Cont".
+  wp_pures. wp_extern.
+  { cbn. apply map_filter_lookup_None_2. right.
+    intros _ _. intros HH; apply HH. eexists; constructor. }
+  iModIntro. cbn. iLeft. iExists _. iSplit; first by eauto.
+  iLeft. do 5 iRight; iLeft. rewrite /proto_readfield /named.
+  do 8 iExists _. iFrame.
+  do 5 (iSplit; first by eauto with lia). iIntros "!>" (? ?) "? ?".
+  iIntros (? ?).
+  iApply wp_value; eauto. iApply "Cont"; eauto. by iFrame.
+Qed.
+
+Lemma alloc_spec E pe (T : ML_proto Σ) θ tg tgnum sz :
+  (0 ≤ sz)%Z →
+  vblock_tag_as_int tg = tgnum →
+  {{{ GC θ }}}
+    (call: &"alloc" with (Val (# tgnum), Val (# sz)))%CE
+      @ (penv_with_prims E pe T); E
+  {{{ θ' γ w, RET w;
+        GC θ' ∗ γ ↦fresh (tg, List.repeat (Lint 0) (Z.to_nat sz)) ∗
+        ⌜repr_lval θ' (Lloc γ) w⌝ }}}.
+Proof.
+  intros. iIntros "HGC Cont".
+  wp_pures. wp_extern.
+  { cbn. apply map_filter_lookup_None_2. right.
+    intros _ _. intros HH; apply HH. eexists; constructor. }
+  iModIntro. cbn. iLeft. iExists _. iSplit; first by eauto.
+  iLeft. do 6 iRight; iLeft. rewrite /proto_alloc /named.
+  do 3 iExists _. iFrame. subst.
+  do 3 (iSplit; first by eauto with lia). iIntros "!>" (? ? ?) "? ? %".
+  iApply wp_value; eauto. iApply "Cont"; eauto. by iFrame.
+Qed.
+
+Lemma alloc_foreign_spec E pe (T : ML_proto Σ) θ a :
+  {{{ GC θ }}}
+    (call: &"alloc_foreign" with (Val (# a)))%CE
+      @ (penv_with_prims E pe T); E
+  {{{ θ' γ w, RET w;
+        GC θ' ∗ γ ↦foreign a ∗
+        ⌜repr_lval θ' (Lloc γ) w⌝ }}}.
+Proof.
+  intros. iIntros "HGC Cont".
+  wp_pures. wp_extern.
+  { cbn. apply map_filter_lookup_None_2. right.
+    intros _ _. intros HH; apply HH. eexists; constructor. }
+  iModIntro. cbn. iLeft. iExists _. iSplit; first by eauto.
+  iLeft. do 7 iRight; iLeft. rewrite /proto_alloc_foreign /named.
+  do 2 iExists _. iFrame.
+  do 2 (iSplit; first by eauto with lia). iIntros "!>" (? ? ?) "? ? %".
+  iApply wp_value; eauto. iApply "Cont"; eauto. by iFrame.
+Qed.
+
+Lemma write_foreign_spec E pe (T : ML_proto Σ) θ w γ a a' :
+  repr_lval θ (Lloc γ) w →
+  {{{ GC θ ∗ γ ↦foreign a }}}
+    (call: &"write_foreign" with (Val w, Val (# a')))%CE
+      @ (penv_with_prims E pe T); E
+  {{{ RET (# 0); GC θ ∗ γ ↦foreign a' }}}.
+Proof.
+  intros. iIntros "(HGC & ?) Cont".
+  wp_pures. wp_extern.
+  { cbn. apply map_filter_lookup_None_2. right.
+    intros _ _. intros HH; apply HH. eexists; constructor. }
+  iModIntro. cbn. iLeft. iExists _. iSplit; first by eauto.
+  iLeft. do 8 iRight; iLeft. rewrite /proto_write_foreign /named.
+  do 5 iExists _. iFrame.
+  do 3 (iSplit; first by eauto with lia). iIntros "!> ? ?".
+  iApply wp_value; eauto. iApply "Cont"; eauto. by iFrame.
+Qed.
+
+Lemma read_foreign_spec E pe (T : ML_proto Σ) θ w γ a :
+  repr_lval θ (Lloc γ) w →
+  {{{ GC θ ∗ γ ↦foreign a }}}
+    (call: &"read_foreign" with (Val w))%CE
+      @ (penv_with_prims E pe T); E
+  {{{ RET (# a); GC θ ∗ γ ↦foreign a }}}.
+Proof.
+  intros. iIntros "(HGC & ?) Cont".
+  wp_pures. wp_extern.
+  { cbn. apply map_filter_lookup_None_2. right.
+    intros _ _. intros HH; apply HH. eexists; constructor. }
+  iModIntro. cbn. iLeft. iExists _. iSplit; first by eauto.
+  iLeft. do 9 iRight. rewrite /proto_read_foreign /named.
+  do 4 iExists _. iFrame.
+  do 3 (iSplit; first by eauto with lia). iIntros "!> ? ?".
+  iApply wp_value; eauto. iApply "Cont"; eauto. by iFrame.
+Qed.
+
+Lemma callback_spec E pe (T : ML_proto Σ) θ w γ f x e lv' w' v' ψ :
+  repr_lval θ (Lloc γ) w →
+  repr_lval θ lv' w' →
+  {{{ GC θ ∗
+      γ ↦clos (f, x, e) ∗
+      lv' ~~ v' ∗
+      (▷ WP (App (ML_lang.Val (RecV f x e)) (ML_lang.Val v')) @ mkPeML ∅ T; E {{ ψ }})
+  }}}
+    (call: &"callback" with (Val w, Val w'))%CE
+      @ (penv_with_prims E pe T); E
+  {{{ θ' vret lvret wret, RET wret;
+        GC θ' ∗
+        ψ vret ∗
+        lvret ~~ vret ∗
+        ⌜repr_lval θ' lvret wret⌝ }}}.
+Proof.
+  intros. iIntros "(? & ? & ? & ?) Cont".
+  wp_pures. wp_extern.
+  { cbn. apply map_filter_lookup_None_2. right.
+    intros _ _. intros HH; apply HH. eexists; constructor. }
+  iModIntro. cbn. iLeft. iExists _. iSplit; first by eauto.
+  iRight. rewrite /proto_callback /named.
+  do 10 iExists _. iFrame.
+  do 4 (iSplit; first by eauto with lia). iIntros "!>" (? ? ? ?) "? ? ? %".
+  iApply wp_value; eauto. iApply "Cont"; eauto. by iFrame.
 Qed.
 
 End Laws.
