theories/interop/prims_proto.v
@@ -3,6 +3,7 @@ From stdpp Require Import strings gmap list.
 From iris.proofmode Require Import proofmode.
 From melocoton Require Import named_props.
 From melocoton.ml_lang Require Import lang_instantiation primitive_laws.
+From melocoton.interop Require Export prims.
 From melocoton.interop Require Import basics_resources gctoken prims.
 
 Section PrimsProto.
@@ -25,7 +26,7 @@ Definition proto_int2val : prim_proto := (λ p vl Φ,
      "HGC" ∷ GC θ ∗
      "->" ∷ ⌜p = Pint2val⌝ ∗
      "->" ∷ ⌜vl = [C_intf.LitV $ C_intf.LitInt $ z]⌝ ∗
-     "Cont" ∷ (∀ w, GC θ -∗ ⌜repr_lval θ (Lint z) w⌝ -∗ Φ w))%I.
+     "Cont" ∷ ▷ (∀ w, GC θ -∗ ⌜repr_lval θ (Lint z) w⌝ -∗ Φ w))%I.
 
 Definition proto_val2int : prim_proto := (λ p vl Φ,
    ∃ θ w z,
@@ -33,7 +34,7 @@ Definition proto_val2int : prim_proto := (λ p vl Φ,
      "->" ∷ ⌜p = Pval2int⌝ ∗
      "->" ∷ ⌜vl = [ w ]⌝ ∗
      "%Hrepr" ∷ ⌜repr_lval θ (Lint z) w⌝ ∗
-     "Cont" ∷ (GC θ -∗ Φ (C_intf.LitV $ C_intf.LitInt $ z)))%I.
+     "Cont" ∷ ▷ (GC θ -∗ Φ (C_intf.LitV $ C_intf.LitInt $ z)))%I.
 
 Definition proto_registerroot : prim_proto := (λ p vl Φ,
    ∃ θ l v w,
@@ -42,7 +43,7 @@ Definition proto_registerroot : prim_proto := (λ p vl Φ,
      "->" ∷ ⌜vl = [ C_intf.LitV $ C_intf.LitLoc $ l ]⌝ ∗
      "Hpto" ∷ l ↦C w ∗
      "%Hrepr" ∷ ⌜repr_lval θ v w⌝ ∗
-     "Cont" ∷ (GC θ -∗ l ↦roots v -∗ Φ (C_intf.LitV $ C_intf.LitInt $ 0)))%I.
+     "Cont" ∷ ▷ (GC θ -∗ l ↦roots v -∗ Φ (C_intf.LitV $ C_intf.LitInt $ 0)))%I.
 
 Definition proto_unregisterroot : prim_proto := (λ p vl Φ,
    ∃ θ l v,
@@ -50,7 +51,7 @@ Definition proto_unregisterroot : prim_proto := (λ p vl Φ,
      "->" ∷ ⌜p = Punregisterroot⌝ ∗
      "->" ∷ ⌜vl = [ C_intf.LitV $ C_intf.LitLoc $ l ]⌝ ∗
      "Hpto" ∷ l ↦roots v ∗
-     "Cont" ∷ (∀w, GC θ -∗ l ↦C w -∗ ⌜repr_lval θ v w⌝ -∗ Φ (C_intf.LitV $ C_intf.LitInt $ 0)))%I.
+     "Cont" ∷ ▷ (∀ w, GC θ -∗ l ↦C w -∗ ⌜repr_lval θ v w⌝ -∗ Φ (C_intf.LitV $ C_intf.LitInt $ 0)))%I.
 
 Definition proto_modify : prim_proto := (λ p vl Φ,
   ∃ θ w i v' w' γ mut tg vs,
@@ -63,9 +64,9 @@ Definition proto_modify : prim_proto := (λ p vl Φ,
     "%Hreprw'" ∷ ⌜repr_lval θ v' w'⌝ ∗
     "%Hi1" ∷ ⌜0 ≤ i⌝%Z ∗
     "%Hi2" ∷ ⌜i < length vs⌝%Z ∗
-    "Cont" ∷ (GC θ -∗
-              γ ↦vblk[mut] (tg, <[Z.to_nat i:=v']> vs) -∗
-              Φ (C_intf.LitV $ C_intf.LitInt $ 0)))%I.
+    "Cont" ∷ ▷ (GC θ -∗
+                 γ ↦vblk[mut] (tg, <[Z.to_nat i:=v']> vs) -∗
+                 Φ (C_intf.LitV $ C_intf.LitInt $ 0)))%I.
 
 Definition proto_readfield : prim_proto := (λ p vl Φ,
    ∃ θ w i γ dq m tg vs,
@@ -76,11 +77,11 @@ Definition proto_readfield : prim_proto := (λ p vl Φ,
      "Hpto" ∷ γ ↦vblk[m]{dq} (tg, vs) ∗
      "%Hi1" ∷ ⌜0 ≤ i⌝%Z ∗
      "%Hi2" ∷ ⌜i < length vs⌝%Z ∗
-     "Cont" ∷ (∀ v' w', GC θ -∗
-                        γ ↦vblk[m]{dq} (tg, vs) -∗
-                        ⌜vs !! (Z.to_nat i) = Some v'⌝ -∗
-                        ⌜repr_lval θ v' w'⌝ -∗
-                        Φ w'))%I.
+     "Cont" ∷ ▷ (∀ v' w', GC θ -∗
+                           γ ↦vblk[m]{dq} (tg, vs) -∗
+                           ⌜vs !! (Z.to_nat i) = Some v'⌝ -∗
+                           ⌜repr_lval θ v' w'⌝ -∗
+                           Φ w'))%I.
 
 Definition proto_alloc : prim_proto := (λ p vl Φ,
    ∃ θ tg sz,
@@ -88,20 +89,20 @@ Definition proto_alloc : prim_proto := (λ p vl Φ,
      "->" ∷ ⌜p = Palloc⌝ ∗
      "->" ∷ ⌜vl = [ C_intf.LitV $ C_intf.LitInt $ vblock_tag_as_int $ tg; C_intf.LitV $ C_intf.LitInt $ sz ]⌝ ∗
      "%Hsz" ∷ ⌜0 ≤ sz⌝%Z ∗
-     "Cont" ∷ (∀ θ' γ w, GC θ' -∗
-                         γ ↦fresh (tg, List.repeat (Lint 0) (Z.to_nat sz)) -∗
-                         ⌜repr_lval θ' (Lloc γ) w⌝ -∗
-                         Φ w))%I.
+     "Cont" ∷ ▷ (∀ θ' γ w, GC θ' -∗
+                            γ ↦fresh (tg, List.repeat (Lint 0) (Z.to_nat sz)) -∗
+                            ⌜repr_lval θ' (Lloc γ) w⌝ -∗
+                            Φ w))%I.
 
 Definition proto_alloc_foreign : prim_proto := (λ p vl Φ,
   ∃ θ a,
     "HGC" ∷ GC θ ∗
     "->" ∷ ⌜p = Pallocforeign⌝ ∗
     "->" ∷ ⌜vl = [ C_intf.LitV (C_intf.LitLoc a) ]⌝ ∗
-    "Cont" ∷ (∀ θ' γ w, GC θ' -∗
-                        γ ↦foreign a -∗
-                        ⌜repr_lval θ' (Lloc γ) w⌝ -∗
-                        Φ w))%I.
+    "Cont" ∷ ▷ (∀ θ' γ w, GC θ' -∗
+                           γ ↦foreign a -∗
+                           ⌜repr_lval θ' (Lloc γ) w⌝ -∗
+                           Φ w))%I.
 
 Definition proto_write_foreign : prim_proto := (λ p vl Φ,
   ∃ θ γ w a a',
@@ -110,9 +111,9 @@ Definition proto_write_foreign : prim_proto := (λ p vl Φ,
     "->" ∷ ⌜vl = [ w; C_intf.LitV (C_intf.LitLoc a') ]⌝ ∗
     "%Hreprw" ∷ ⌜repr_lval θ (Lloc γ) w⌝ ∗
     "Hpto" ∷ γ ↦foreign a ∗
-    "Cont" ∷ (GC θ -∗
-              γ ↦foreign a' -∗
-              Φ (C_intf.LitV (C_intf.LitInt 0))))%I.
+    "Cont" ∷ ▷ (GC θ -∗
+                 γ ↦foreign a' -∗
+                 Φ (C_intf.LitV (C_intf.LitInt 0))))%I.
 
 Definition proto_read_foreign : prim_proto := (λ p vl Φ,
   ∃ θ γ w a,
@@ -121,9 +122,9 @@ Definition proto_read_foreign : prim_proto := (λ p vl Φ,
     "->" ∷ ⌜vl = [ w ]⌝ ∗
     "%Hreprw" ∷ ⌜repr_lval θ (Lloc γ) w⌝ ∗
     "Hpto" ∷ γ ↦foreign a ∗
-    "Cont" ∷ (GC θ -∗
-              γ ↦foreign a -∗
-              Φ (C_intf.LitV (C_intf.LitLoc a))))%I.
+    "Cont" ∷ ▷ (GC θ -∗
+                 γ ↦foreign a -∗
+                 Φ (C_intf.LitV (C_intf.LitLoc a))))%I.
 
 Definition proto_callback (E : coPset) (T : ML_proto) : prim_proto := (λ p vl Φ,
   ∃ θ w γ w' lv' v' f x e ψ,
@@ -135,12 +136,12 @@ Definition proto_callback (E : coPset) (T : ML_proto) : prim_proto := (λ p vl �
     "%Hreprw'" ∷ ⌜repr_lval θ lv' w'⌝ ∗
     "Hsim'" ∷ lv' ~~ v' ∗
     "WPcallback" ∷ ▷ WP (App (Val (RecV f x e)) (Val v')) @ mkPeML ∅ T ; E {{ ψ }} ∗
-    "Cont" ∷ (∀ θ' vret lvret wret,
-                GC θ' -∗
-                ψ vret -∗
-                lvret ~~ vret -∗
-                ⌜repr_lval θ' lvret wret⌝ -∗
-                Φ wret))%I.
+    "Cont" ∷ ▷ (∀ θ' vret lvret wret,
+                   GC θ' -∗
+                   ψ vret -∗
+                   lvret ~~ vret -∗
+                   ⌜repr_lval θ' lvret wret⌝ -∗
+                   Φ wret))%I.
 
 (* non-callbacks primitives *)
 Definition proto_base_prims : prim_proto := (λ p vl Φ,
@@ -169,3 +170,9 @@ Definition proto_prims_in_C E (T : ML_proto) : C_proto := (λ f vs Φ,
 )%I.
 
 End PrimsProto.
+
+(* TODO: move? *)
+Notation mkPeML p T := ({| penv_prog := p; penv_proto := T |} : prog_environ ML_lang (_ : gFunctors)).
+Notation prim_proto Σ := (prim -d> list C_intf.val -d> (C_intf.val -d> iPropO Σ) -d> iPropO Σ).
+Notation C_proto Σ := (string -d> list C_intf.val -d> (C_intf.val -d> iPropO Σ) -d> iPropO Σ).
+Notation ML_proto Σ := (string -d> list ML_lang.val -d> (ML_lang.val -d> iPropO Σ) -d> iPropO Σ).
